NoLoc.v
@@ -8,91 +8,91 @@ From Elo Require Import Access.
 
 Inductive NoLoc : tm -> Prop :=
   | noloc_unit :
-      NoLoc TM_Unit
+      NoLoc <{ unit }> 
 
   | noloc_num : forall n,
-      NoLoc (TM_Num n)
+      NoLoc <{ N n }>
 
-  | noloc_new : forall t,
+  | noloc_new : forall T t,
       NoLoc t ->
-      NoLoc (TM_New t)
+      NoLoc <{ new T t }>
 
   | noloc_load : forall t,
       NoLoc t ->
-      NoLoc (TM_Load t)
+      NoLoc <{ *t }>
 
   | noloc_asg : forall t1 t2,
       NoLoc t1 ->
       NoLoc t2 ->
-      NoLoc (TM_Asg t1 t2)
+      NoLoc <{ t1 = t2 }>
 
-  | noloc_fun : forall x X t,
+  | noloc_fun : forall x Tx t,
       NoLoc t ->
-      NoLoc (TM_Fun x X t)
+      NoLoc <{ fn x Tx --> t }>
 
   | noloc_call : forall t1 t2,
       NoLoc t1 ->
       NoLoc t2 ->
-      NoLoc (TM_Call t1 t2)
+      NoLoc <{ call t1 t2 }>
 
   | noloc_seq : forall t1 t2,
       NoLoc t1 ->
       NoLoc t2 ->
-      NoLoc (TM_Seq t1 t2)
+      NoLoc <{ t1; t2 }>
 
   | noloc_spawn : forall t,
       NoLoc t ->
-      NoLoc (TM_Spawn t)
+      NoLoc <{ spawn t }>
   .
 
 Inductive SpawnNoLoc : tm -> Prop :=
   | spawn_noloc_unit :
-      SpawnNoLoc TM_Unit
+      SpawnNoLoc <{ unit }> 
 
   | spawn_noloc_num : forall n,
-      SpawnNoLoc (TM_Num n)
+      SpawnNoLoc <{ N n }>
 
-  | spawn_noloc_loc : forall ad,
-      SpawnNoLoc (TM_Loc ad)
+  | spawn_noloc_loc : forall ad T,
+      SpawnNoLoc <{ &ad :: T }>
 
-  | spawn_noloc_new : forall t,
+  | spawn_noloc_new : forall T t,
       SpawnNoLoc t ->
-      SpawnNoLoc (TM_New t)
+      SpawnNoLoc <{ new T t }>
 
   | spawn_noloc_load : forall t,
       SpawnNoLoc t ->
-      SpawnNoLoc (TM_Load t)
+      SpawnNoLoc <{ *t }>
 
   | spawn_noloc_asg : forall t1 t2,
       SpawnNoLoc t1 ->
       SpawnNoLoc t2 ->
-      SpawnNoLoc (TM_Asg t1 t2)
+      SpawnNoLoc <{ t1 = t2 }>
 
-  | spawn_noloc_fun : forall x X t,
+  | spawn_noloc_fun : forall x Tx t,
       SpawnNoLoc t ->
-      SpawnNoLoc (TM_Fun x X t)
+      SpawnNoLoc <{ fn x Tx --> t }>
 
   | spawn_noloc_call : forall t1 t2,
       SpawnNoLoc t1 ->
       SpawnNoLoc t2 ->
-      SpawnNoLoc (TM_Call t1 t2)
+      SpawnNoLoc <{ call t1 t2 }>
 
   | spawn_noloc_seq : forall t1 t2,
       SpawnNoLoc t1 ->
       SpawnNoLoc t2 ->
-      SpawnNoLoc (TM_Seq t1 t2)
+      SpawnNoLoc <{ t1; t2 }>
 
   | spawn_noloc_spawn : forall t,
       NoLoc t ->
-      SpawnNoLoc (TM_Spawn t)
+      SpawnNoLoc <{ spawn t }>
   .
 
 Local Ltac inversion_spawn_noloc :=
   match goal with
   | H : SpawnNoLoc TM_Unit        |- _ => inversion H; subst; clear H
   | H : SpawnNoLoc (TM_Num _)     |- _ => inversion H; subst; clear H
-  | H : SpawnNoLoc (TM_Loc _)     |- _ => inversion H; subst; clear H
-  | H : SpawnNoLoc (TM_New _)     |- _ => inversion H; subst; clear H
+  | H : SpawnNoLoc (TM_Ref _ _)   |- _ => inversion H; subst; clear H
+  | H : SpawnNoLoc (TM_New _ _)   |- _ => inversion H; subst; clear H
   | H : SpawnNoLoc (TM_Load _)    |- _ => inversion H; subst; clear H
   | H : SpawnNoLoc (TM_Asg _ _)   |- _ => inversion H; subst; clear H
   | H : SpawnNoLoc (TM_Fun _ _ _) |- _ => inversion H; subst; clear H
@@ -101,14 +101,14 @@ Local Ltac inversion_spawn_noloc :=
   | H : SpawnNoLoc (TM_Spawn _)   |- _ => inversion H; subst; clear H
   end.
 
-Local Lemma spawn_noloc_subst : forall x X t t',
-  SpawnNoLoc (TM_Fun x X t) ->
+Local Lemma spawn_noloc_subst : forall x Tx t t',
+  SpawnNoLoc <{ fn x Tx --> t }> ->
   SpawnNoLoc t' ->
   SpawnNoLoc ([x := t'] t).
 Proof.
   intros * H ?. inversion H; clear H; subst.
   induction t; eauto using SpawnNoLoc; simpl; 
-  try (destruct String.eqb; trivial);
+  try (destruct String.string_dec; trivial);
   inversion_spawn_noloc; eauto using SpawnNoLoc.
 Qed.
 
@@ -116,7 +116,7 @@ Local Lemma spawn_noloc_alloc : forall m t t' v,
   SpawnNoLoc t ->
   memory_property SpawnNoLoc m ->
   t --[EF_Alloc (length m) v]--> t' ->
-  memory_property SpawnNoLoc (add m v).
+  memory_property SpawnNoLoc (m +++ v).
 Proof.
   intros. assert (SpawnNoLoc v).
   { induction_step; inversion_spawn_noloc; eauto. }
@@ -126,8 +126,8 @@ Qed.
 Local Lemma spawn_noloc_store : forall m t t' ad v,
   memory_property SpawnNoLoc m ->
   SpawnNoLoc t ->
-  t --[EF_Store ad v]--> t' ->
-  memory_property SpawnNoLoc (set m ad v).
+  t --[EF_Write ad v]--> t' ->
+  memory_property SpawnNoLoc m[ad <- v].
 Proof.
   intros. assert (SpawnNoLoc v).
   { induction_step; inversion_spawn_noloc; eauto. }
@@ -209,8 +209,7 @@ Lemma noloc_then_not_access : forall m t ad,
   ~ access m t ad.
 Proof.
   intros * Hnl. induction t; inversion Hnl; subst;
-  eauto using not_access_new, not_access_load, not_access_asg, not_access_fun,
-    not_access_call, not_access_seq;
+  eapply not_access_iff; eauto using not_access;
   intros ?; inversion_access.
 Qed.
 
