Makefile
@@ -2,22 +2,24 @@
 
 COQC= coqc -Q . Elo
 
-main: core
-	$(COQC) Compat.v
-	$(COQC) AccessProp.v
-	$(COQC) NoLoc.v
-	$(COQC) Disjoint.v
+all: soundness safety 
 
 core:
 	$(COQC) Util.v
 	$(COQC) Array.v
 	$(COQC) Map.v
 	$(COQC) Core.v
+	$(COQC) Access.v
 
 soundness: core
-	$(COQC) Access.v
 	$(COQC) References.v
 	$(COQC) Soundness.v
+
+safety: core
+	$(COQC) Compat.v
+	$(COQC) AccessProp.v
+	$(COQC) NoLoc.v
+	$(COQC) Disjoint.v
 
 clean:
 	rm -f .lia.cache .*.aux *.vo *.vok *.vos *.glob
